\documentclass[twoside,11pt]{article}
\usepackage[left=1in, right=1in, top=1in, bottom=1in]{geometry}
\usepackage{amsmath}
\usepackage{amssymb}
\usepackage{amsfonts}
\usepackage{mathtools}
\usepackage{amsthm}
\usepackage{fancyhdr}
\usepackage{enumitem}
\usepackage{siunitx}
\usepackage{booktabs}
\usepackage[hidelinks]{hyperref}
\usepackage{sectsty}
\usepackage{mathrsfs} % mathscr
\usepackage{tikz}
\usepackage{pgfplots}
\usepackage{multicol}
\usepackage{listings}
% \usepackage{amsart}
\usepackage{fontspec}
\usepackage{soul}


% allow H option of figure
\usepackage{float}

% math font (libertine)
\usepackage{libertinus-otf}

% braket
\usepackage{braket}

% physics
% \usepackage{physics}

% define latin modern font environment
\newcommand{\lms}{\fontfamily{lmss}\selectfont} % Latin Modern Roman
% \newcommand{\lmss}{\fontfamily{lmss}\selectfont} % Latin Modern Sans
% \newcommand{\lmss}{\fontfamily{lmtt}\selectfont} % Latin Modern Mono

% % change mathcal shape
% \usepackage[mathcal]{eucal}


% define math operators
\newcommand{\FF}{\mathbb{F}}
\newcommand{\RR}{\mathbb{R}}
\newcommand{\NN}{\mathbb{N}}
\newcommand{\ZZ}{\mathbb{Z}}
\newcommand{\QQ}{\mathbb{Q}}
\newcommand{\XX}{\mathbb{Y}}
\newcommand{\CL}{\mathcal{L}}
% \renewcommand{\d}{\mathrm{d}}
\renewcommand*\d{\mathop{}\!\mathrm{d}}
\DeclareMathOperator*{\argmax}{arg\,max}
\DeclareMathOperator*{\argmin}{arg\,min}
\DeclareMathOperator{\im}{im}
\DeclareMathOperator{\id}{id}
\DeclareMathOperator{\erf}{erf}
\renewcommand{\mod}[1]{\ (\mathrm{mod}\ #1)}

% section font style
\sectionfont{\sffamily\Large}
\subsectionfont{\sffamily\normalsize}
\subsubsectionfont{\bf}

% line spreading and break
\hyphenpenalty=5000
\tolerance=20
\setlength{\parindent}{0em}
\setlength\parskip{0.5em}
\allowdisplaybreaks
\linespread{0.9}

% enumerate settings
% no break before enumerate
\setlist[enumerate]{itemsep=2pt,topsep=2pt}

% theorem
% latex theorem
% definition style
\theoremstyle{definition}
\newtheorem{theorem}{Theorem}[subsection]
\newtheorem{axiom}{Axiom}[section]
\newtheorem{definition}{Definition}[section]
\newtheorem{example}{Example}[section]
\newtheorem{question}{Question}[section]
\newtheorem{exercise}{Exercise}[section]
\newtheorem*{exercise*}{Exercise}
\newtheorem{lemma}{Lemma}[section]
\newtheorem{proposition}{Proposition}[section]
\newtheorem{corollary}{Corollary}[section]
\newtheorem*{theorem*}{Theorem}
\newtheorem{problem}{Problem}
% remark style
\theoremstyle{remark}
\newtheorem*{remark}{Remark}
\newtheorem*{solution}{Solution}
\newtheorem*{claim}{Claim}


% paragraph indent
\setlength{\parindent}{0em}
\setlength\parskip{0.5em}

\newcommand\Code{PHY5410 FA22}
\newcommand\Ass{HW08}
\newcommand\name{Haoran Sun}
\newcommand\mail{haoransun@link.cuhk.edu.cn}

\title{{\lms \Code \ \Ass}}
\author{\lms \name \ (\href{mailto:\mail}{\mail})}
\date{\sffamily \today}

\makeatletter
% \let\Title\@title
\let\theauthor\@author
\let\thedate\@date

\fancypagestyle{plain}{%
    \fancyhf{}
    \lhead{\sffamily \Ass}
    \rhead{\sffamily \name}
    \rfoot{\sffamily\thepage}

    % # 页脚自定义
    \fancyfoot[L]{
        \begin{minipage}[c]{0.06\textwidth}
            \includegraphics[height=7.5mm]{logo2.png}
        \end{minipage}
    }
}
\fancypagestyle{title}{%
    \fancyhf{}
    \renewcommand{\headrulewidth}{0pt}
    % \lhead{\Title}
    % \rhead{\theauthor}
    \rfoot{\sffamily\thepage}

    % # 页脚自定义
    \fancyfoot[L]{
        \begin{minipage}[c]{0.06\textwidth}
            \includegraphics[height=7.5mm]{logo2.png}
        \end{minipage}
    }
}
\fancyfootoffset[L]{0.3cm}

% re-define title format
\makeatletter
\renewcommand{\maketitle}{\bgroup\setlength{\parindent}{0pt}
\begin{flushleft}
  \textbf{\Large\@title}

  \@author
\end{flushleft}\egroup
}
\makeatother

\pagestyle{plain}

% lstlisting settings
\lstset{
    basicstyle=\linespread{0.7}\footnotesize,
    breaklines=true,
    basewidth=0.5em
}


\begin{document}
\maketitle
\thispagestyle{title}
% \begin{multicols*}{2}

% \begin{remark}
%     $V_\epsilon(x)$ is used to denote a $\epsilon$-neighborhood
%     \begin{align*}
%         V_\epsilon(x) = B_\epsilon(x)\setminus\{x\}
%     \end{align*}
% \end{remark}

\begin{problem}[16.5]
The first-order transition probability of a ground state to the $n$th excited state is written in the form
\begin{align*}
    P_{0n}(t) &= |\braket{n, t|\psi, t}|^2
    = \left|
    \frac{1}{\hbar}
    \int_{t_0}^t\d t'\ e^{i\omega_{n0}t'}\braket{n|V(t')|0}
    \right|^2
\end{align*}
where $\omega_{n0} = (E_n - E_0)/\hbar$.
Since $t_0 < t_1$ and $t>t_2$, we have
\begin{align*}
    \int_{t_0}^t\d t'\ e^{i\omega_{n0}t'}\braket{n|V(t')|0}
    &= 
    \int_{t_1}^{t_2}\d t'\ e^{i\omega_{n0}t'}\braket{n|V(t')|0}
    = 
    \braket{n|x|0}
    \int_{t_1}^{t_2}\d t'\ e^{i\omega_{n0}t'}(-D\cos\Omega t)
\end{align*}
Easy to prove that
\begin{align*}
    \braket{n|x|0} &= \sqrt{\frac{\hbar}{2m\omega}}\delta_{n1}
\end{align*}
and
\begin{align*}
    \int_{t_1}^{t_2} \d t'\ e^{i\omega_{n0}t'}\cos\Omega t'
    &= 
    \frac{1}{\omega_{n0}^2 - \Omega^2}(
        \omega_{n0}\cos\omega_{n0}t\cos\Omega - 
        \Omega\cos\omega_{n0}t\sin\Omega t
    )|_{t_1}^{t_2} \\
    &+\ i
    \frac{1}{\Omega^2 - \omega_{n0}^2}(
        \omega_{n0}\cos\omega_{n0}t\cos\Omega t +
        \Omega\sin\omega_{n0}t\sin\Omega t
    )|_{t_1}^{t_2}
\end{align*}
Hence we can calculate the transition probability.
\begin{align*}
    P_{0n}(t) &= \frac{D^2}{2m\omega\hbar}\left|
        \int_{t_1}^{t_2}\d t'\
        e^{i\omega_{n0}t'}\cos\Omega t'
    \right|^2\delta_{n1}
\end{align*}
Note that $P_{0n}(t)=0$ $\forall n \geq 2$.
\end{problem}



\begin{problem}[16.7]
The wave functions for the old ground state and the new ground state are
\begin{align*}
    \psi(x) &= \frac{\sqrt{m\lambda}}{\hbar}\exp (-m\lambda|x|/\hbar^2)\quad
    \psi'(x) = \frac{\sqrt{m\mu}}{\hbar}\exp (-m\mu|x|/\hbar^2)\quad
\end{align*}
Hence the transition probability is
\begin{align*}
    \braket{\psi'|\psi} &= 2\int_0^\infty \frac{m}{\hbar^2}
    \sqrt{\lambda\mu}\exp[-m(\lambda+\mu)|x|/\hbar^2] = \frac{2\sqrt{\lambda\mu}}{\lambda+\mu}
\end{align*}
\end{problem}



\begin{problem}[16.10]
Since
\begin{align*}
    [\dot{x}, x] &= \left[\frac{1}{i\hbar}(xH-Hx), x\right] = \frac{1}{i\hbar}
    (2xHx - Hx^2 - x^2H)
\end{align*}
Notice that
\begin{align*}
    \braket{a|xHx|a} &= \sum_n\braket{a|x|n}\braket{n|Hx|a}
    = \sum_n E_n|\braket{n|x|a}|^2\\
    \braket{a|Hx^2|a} &= \sum_n \braket{a|Hx|n}\braket{n|x|a} = \sum_n E_a|\braket{n|x|a}|^2\\
    \braket{a|x^2H|a} &= \sum_n \braket{a|x|n}\braket{n|xH|a} = \sum_n E_a|\braket{n|x|a}|^2
\end{align*}
Therefore
\begin{align*}
    \braket{a|[\dot{x}, x]|a} &= \frac{2}{i\hbar}\sum_n (E_n-E_a)|\braket{n|x|a}|^2
\end{align*}
For $H = p^2/2m + m\omega^2 x/2m$, we have
\begin{align*}
    \dot{x} = \frac{\partial }{\partial p}H = \frac{p}{m}
    \Rightarrow [\dot{x}, x] = -\frac{i\hbar}{m}
\end{align*}
Therefore
\begin{align*}
    \sum_n(E_n-E_a)|\braket{n|x|a}|^2 &= \frac{\hbar^2}{2m}
\end{align*}


\end{problem}


% \end{multicols*}
\end{document}

